ROOT
@@ -5,14 +5,16 @@
 *)
 session "repliss" = "HOL" +
   options [document = pdf, document_output = "output"]
-  theories [document = false]
+  sessions 
+    "HOL-Library"
+ (* theories [document = false]
     "~~/src/HOL/Library/FSet"
     "~~/src/HOL/Eisbach/Eisbach"
     "~~/src/HOL/Library/Sublist"
     "~~/src/HOL/Library/LaTeXsugar"
     "~~/src/HOL/Library/OptionalSugar"
     "~~/src/HOL/Library/Multiset"
-    "~~/src/HOL/Library/Option_ord"
+    "~~/src/HOL/Library/Option_ord" *)
   theories [show_question_marks = false, names_short]
     invariant_simps
   document_files
